Classes/Monad/MonadJoin.v
@@ -9,3 +9,15 @@ Class MonadJoin M {MM : Monad M} : Type := {
 Hint Rewrite @mjoin_return : monads.
 
 Infix "<⊔>" := mjoin (at level 40).
+
+Definition mjoin_option A {JA : Joinable A A} : option A → option A → option A :=
+  λ m1 : option A, λ m2 : option A,
+    match m1, m2 with
+    | Some x, Some y => Some (x ⊔ y)
+    | _, _ => None
+    end.
+
+Instance option_monadjoin : MonadJoin option.
+Proof.
+  split with mjoin_option. reflexivity.
+Defined.
